git/leanprover/lean4/src/Init/Core.lean
@@ -89,6 +89,12 @@ class ForIn (m : Type u₁ → Type u₂) (ρ : Type u) (α : outParam (Type v))
 
 export ForIn (forIn)
 
+class ForIn' (m : Type u₁ → Type u₂) (ρ : Type u) (α : outParam (Type v)) (d : outParam $ Membership α ρ) where
+  forIn' {β} [Monad m] (x : ρ) (b : β) (f : (a : α) → a ∈ x → β → m (ForInStep β)) : m β
+
+export ForIn' (forIn')
+
+
 /- Auxiliary type used to compile `do` notation. -/
 inductive DoResultPRBC (α β σ : Type u) where
   | «pure»     : α → σ → DoResultPRBC α β σ
@@ -418,13 +424,13 @@ end Decidable
 
 section
 variable {p q : Prop}
-@[inline] def  decidableOfDecidableOfIff (hp : Decidable p) (h : p ↔ q) : Decidable q :=
+@[inline] def  decidable_of_decidable_of_iff [hp : Decidable p] (h : p ↔ q) : Decidable q :=
   if hp : p then
     isTrue (Iff.mp h hp)
   else
     isFalse fun hq => absurd (Iff.mpr h hq) hp
 
-@[inline] def  decidableOfDecidableOfEq (hp : Decidable p) (h : p = q) : Decidable q :=
+@[inline] def  decidable_of_decidable_of_eq [hp : Decidable p] (h : p = q) : Decidable q :=
   h ▸ hp
 end
 
