git/FWuermse/lean-postgres/examples/open-connection/Main.lean
@@ -1,6 +1,7 @@
 import Postgres
 
-open Connection
+open Connect
+open Query
 
 def zeroToSpace : UInt8 → UInt8
 | 0 => 32
@@ -8,7 +9,7 @@ def zeroToSpace : UInt8 → UInt8
 
 def main : IO Unit := do
   let conn ← openConnection "localhost" "5432" "postgres" "postgres" "pw"
-  let resp ← sendQuery conn "SELECT * FROM pf;"
-  IO.println "TEST"
+  let query := SELECT "pilot", "flugzeug" FROM "pf";
+  let resp ← sendQuery conn query
   IO.println $ String.fromUTF8Unchecked $ List.toByteArray $ List.map zeroToSpace resp.toList
   conn.close
