git/UlisseMini/ladoneright/lakefile.lean
@@ -1,6 +1,0 @@
-import Lake
-open Lake DSL
-
-package LinearAlgebraDoneRight {
-  -- add configuration options here
-}
