git/UlisseMini/ladoneright/README.md
@@ -1,4 +1,0 @@
-# ladoneright
-
-Theorems from axler's "Linear Algebra Done Right" in Lean4.
-Built because people on the internet said I'm not being rigorous
